nola/iris/ofe.v
@@ -3,12 +3,15 @@
 From nola Require Export prelude.
 From iris.algebra Require Import ofe cmra.
 From iris.bi Require Import bi.
+From iris.base_logic Require Import iprop.
 
 Implicit Type PROP : bi.
 
+Notation oiapp F Σ := (oFunctor_apply F (iProp Σ)).
+Notation riapp F Σ := (rFunctor_apply F (iProp Σ)).
 Module OfeNotation.
-  Notation "F $o x" := (oFunctor_apply F x) (at level 20, right associativity).
-  Notation "F $r x" := (rFunctor_apply F x) (at level 20, right associativity).
+  Notation "F $o Σ" := (oiapp F Σ) (at level 20, right associativity).
+  Notation "F $r Σ" := (riapp F Σ) (at level 20, right associativity).
 End OfeNotation.
 
 (** [▷] on [later PROP] *)
